\part{Schwarzschild spacetime}

\chapter{Schwarzschild metric}

    Consider a spherically symmetric source. We study the region outside the source, in which the spacetime is empty and the energy-momentum tensor vanishes $T_{\mu\nu} = 0$. Einstein's field equation becomes 
    \begin{equation*}
        R_{\mu\nu} = 0 ~.
    \end{equation*}
    \begin{proof}
        In fact, computing the trace of~\eqref{fieldeq} in the vacuum
        \begin{equation*}
            0 = g^{\mu\nu} R_{\mu\nu} - \frac{1}{2} \underbrace{g^{\mu\nu} g_{\mu\nu}}_4 R = R - 2 R = - R ~.
        \end{equation*}
        Therefore $R = 0$ and the Einstein's field equations become
        \begin{equation*}
            0 = G_{\mu\nu} = R_{\mu\nu} - \frac{1}{2} \underbrace{R}_0 g_{\mu\nu} = R_{\mu\nu} ~.
        \end{equation*}
    \end{proof}

    The general solution will depend on free parameters which depend on the region inside the source $T_{\mu\nu} \neq 0$. However, we can use spacetime symmetries to reduce to a one-parameter family. 

\section{Isometries}

    Since the general solution is too difficult to compute, we assume isometries, which are spacetime symmetries, associated to Killing vectors, i.e.~vectors $K$ such that 
    \begin{equation*}
        \pounds_K g = 0 ~.
    \end{equation*}

    In our situation, good guesses could be staticity and spherical symmetry. 

    We require that the metric is static, even though the source loses energy, so that there exists a timelike Killing vector $K_{t}$ 
    \begin{equation*}
        \pounds_{K_{t}} g = 0~, \quad g(K_{t}, K_{t}) < 0 ~,
    \end{equation*}
    with a coordinate $t$ such that 
    \begin{equation*}
        K_{t} = \pdv{}{t} ~.
    \end{equation*}

    Moreover, we require that the metric is spherical symmetric, even though the source is nnot really a sphere. This means that there exists $3$ spacelike Killing vector $K_{i}$ 
    \begin{equation*}
        \pounds_{K_{i}} g = 0~, \quad g(K_{i}, K_{i}) > 0 ~,
    \end{equation*}
    with a coordinate $t$ such that 
    \begin{equation*}
        K_{i} = \pdv{}{\theta_i} ~.
    \end{equation*}
    where $i = 1,2,3$. By a theorem, they form a Lie algebra equals to the rotations around the source center
    \begin{equation*}
        [K_i, K_j] = \epsilon_{ijk} K_k ~.
    \end{equation*}
    They would also conserve in time, since coordinates does, which means that they commute with $K_t$
    \begin{equation*}
        [K_i, K_t] = 0 ~.
    \end{equation*}
    We assume also that they are orthogonal to $K_t$, i.e.~spacelike vectors orthogonal to timelike vectors. In this way, the metric is in diagonal form. 

    We have found the same situation of a sphere. Therefore, we can use polar coordinates $(r, \theta, \phi)$ on surfaces at constant $t$. The line element assume a diagonal form 
    \begin{equation*}
        ds^2 = - A(r) dt^2 + B(r) dr^2 + C(r) d\Omega^2 = - A(r) dt^2 + B(r) dr^2 + C(r) (d\theta^2 + \sin^2 \theta d\phi^2) ~.
    \end{equation*}
    where $A(r)$, $B(r)$, $C(r)$ are functions of $r$ and $d \Omega^2 = d\theta^2 + \sin^2 \theta d\phi^2$ is an element of solid angle.

    Since we have the freedom to rescale $r$, we reparametrised in order to intepret it as the areal radius. Therefore, we choose $C(r) = r^2$. This can be seen if we restrict to the submanifold (sphere) $\mathcal S$ with constant $t$ and $r$. In fact, its area is 
    \begin{equation*}
        4\pi r^2 = A(\mathcal S) = \int_0^\pi d\theta \int_0^{2\pi} d\phi~ \sqrt{g_{\theta \phi}} = \int_0^\pi d\theta \int_0^{2\pi} d\phi~ \sin \theta C(r) = 4 \pi C(r) ~.
    \end{equation*}
    Hence $C(r) = r^2$. So far, the line element is 
    \begin{equation*}
        ds^2 = - A(r) dt^2 + B(r) dr^2 + r^2 d\Omega^2 ~.
    \end{equation*}

    As a consequence of isometries, we can define the domain of the chart $(t, r,\theta, \phi)$. Time-translation invariance means $t \in (-\infty, \infty)$ and the foliation of spatial volumes into $2$-dimensional spheres means $\theta \in [0, \pi]$ and $\phi \in [0, 2 \pi]$. 

    However, it is important to highlight that Einstein's field equation, unlike Maxwell ones, not only determine the metric tensor but also the manifold on which it exists. Therefore, about the coordinate $r$ and its domain, we cannot say any further, they are defined by those equations.

    Notice that the proper length of the radius of a sphere is
    \begin{equation*}
        R(r) = \int_0^r dx \sqrt{g_{rr}} = \int_0^r dx \sqrt{B(x)} ~.
    \end{equation*}
    This means that if $B(r) \neq 1$, the spacetime outside the source is curved. 

\section{Einstein's field equations}

    Now, we compute the Einstein's field equations. 

    The metric is 
    \begin{equation*}
        g_{\mu\nu} = \begin{bmatrix}
            A & 0 & 0 & 0 \\
            0 & B & 0 & 0 \\
            0 & 0 & r^2 & 0 \\
            0 & 0 & 0 & r^2 \sin^2 \theta \\
        \end{bmatrix} ~,
    \end{equation*}
    whereas its inverse is 
    \begin{equation*}
        g^{\mu\nu} = \begin{bmatrix}
            \frac{1}{A} & 0 & 0 & 0 \\
            0 & \frac{1}{B} & 0 & 0 \\
            0 & 0 & \frac{1}{r^2} & 0 \\
            0 & 0 & 0 & \frac{1}{r^2 \sin^2 \theta} \\
        \end{bmatrix} ~.
    \end{equation*}

    The derivative with respect to $r$ is 
    \begin{equation*}
        g_{\mu\nu, 1} = \begin{bmatrix}
            A' & 0 & 0 & 0 \\
            0 & B' & 0 & 0 \\
            0 & 0 & 2 r & 0 \\
            0 & 0 & 0 & 2 r \sin^2 \theta \\
        \end{bmatrix} ~,
    \end{equation*}
    whereas its inverse is 
    \begin{equation*}
        g_{\mu\nu, 2} = \begin{bmatrix}
            0 & 0 & 0 & 0 \\
            0 & 0 & 0 & 0 \\
            0 & 0 & 0 & 0 \\
            0 & 0 & 0 & 2 r^2 \sin \theta \cos \theta \\
        \end{bmatrix} ~.
    \end{equation*}

    The Christoffel symbols induced by the metric are
    \begin{equation*}
        \Gamma^k_{ij} = \frac{1}{2} g^{kl} (g_{il,j} + g_{jl,i} - g_{ij,l}) ~.
    \end{equation*}

    \begin{proof}
        The $0$-th Christoffel symbols are
        \begin{equation*}
            \Gamma^0_{00} = \frac{1}{2} g^{0l} (g_{0l,0} + g_{0l,0} - g_{00,l}) = \frac{1}{2} g^{00} (g_{00,0} + g_{00,0} - g_{00,0}) = 0 ~,
        \end{equation*}

        \begin{equation*}
            \Gamma^0_{11} = \frac{1}{2} g^{0l} (g_{1l,1} + g_{1l,1} - g_{11,l}) =  \frac{1}{2} g^{00} (g_{10,1} + g_{10,1} - g_{11,0}) = 0 ~,
        \end{equation*}

        \begin{equation*}
            \Gamma^0_{22} = \frac{1}{2} g^{0l} (g_{2l,2} + g_{2l,2} - g_{22,l}) =  \frac{1}{2} g^{00} (g_{20,2} + g_{20,2} - g_{22,0}) = 0 ~,
        \end{equation*}

        \begin{equation*}
            \Gamma^0_{33} = \frac{1}{2} g^{0l} (g_{3l,3} + g_{3l,3} - g_{33,l}) =  \frac{1}{2} g^{00} (g_{30,3} + g_{30,3} - g_{33,0}) = 0 ~,
        \end{equation*}

        \begin{equation*}
            \Gamma^0_{01} = \Gamma^0_{10} = \frac{1}{2} g^{0l} (g_{1l,0} + g_{0l,1} - g_{10,l}) = \frac{1}{2} \underbrace{g^{00}}_{\frac{1}{A}} (g_{10,0} + \underbrace{g_{00,1}}_{A'} - g_{10,0}) = \frac{A'}{2A} ~,
        \end{equation*}

        \begin{equation*}
            \Gamma^0_{02} = \Gamma^0_{20} = \frac{1}{2} g^{0l} (g_{2l,0} + g_{0l,2} - g_{20,l}) = \frac{1}{2} g^{00} (g_{20,0} + g_{00,2} - g_{20,0}) = 0 ~,
        \end{equation*}

        \begin{equation*}
            \Gamma^0_{03} = \Gamma^0_{30} = \frac{1}{2} g^{0l} (g_{3l,0} + g_{0l,3} - g_{30,l}) = \frac{1}{2} g^{00} (g_{30,0} + g_{00,3} - g_{30,0}) = 0 ~,
        \end{equation*}

        \begin{equation*}
            \Gamma^0_{12} = \Gamma^0_{21} = \frac{1}{2} g^{0l} (g_{2l,1} + g_{1l,2} - g_{21,l}) = \frac{1}{2} g^{00} (g_{20,1} + g_{10,2} - g_{21,0}) = 0 ~,
        \end{equation*}

        \begin{equation*}
            \Gamma^0_{13} = \Gamma^0_{31} = \frac{1}{2} g^{0l} (g_{3l,1} + g_{1l,3} - g_{31,l}) = \frac{1}{2} g^{00} (g_{30,1} + g_{10,3} - g_{31,0}) ~,
        \end{equation*}

        \begin{equation*}
            \Gamma^0_{23} = \Gamma^0_{32} = \frac{1}{2} g^{0l} (g_{3l,2} + g_{2l,3} - g_{32,l}) = \frac{1}{2} g^{00} (g_{30,2} + g_{20,3} - g_{32,0}) = 0 ~.
        \end{equation*}

        The $1$-st Christoffel symbols are 
        \begin{equation*}
            \Gamma^1_{00} = \frac{1}{2} g^{1l} (g_{0l,0} + g_{0l,0} - g_{00,l}) =  \frac{1}{2} \underbrace{g^{11}}_{\frac{1}{B}} (g_{01,0} + g_{01,0} - \underbrace{g_{00,1}}_{A'}) = - \frac{A'}{2B} ~,
        \end{equation*}

        \begin{equation*}
            \Gamma^1_{11} = \frac{1}{2} g^{1l} (g_{1l,1} + g_{1l,1} - g_{11,l}) =  \frac{1}{2} \underbrace{g^{11}}_{\frac{1}{B}} (\underbrace{g_{11,1}}_{B'} + g_{11,1} - g_{11,1}) = \frac{B'}{2B} ~,
        \end{equation*}

        \begin{equation*}
            \Gamma^1_{22} = \frac{1}{2} g^{1l} (g_{2l,2} + g_{2l,2} - g_{22,l}) =  \frac{1}{2} \underbrace{g^{11}}_{\frac{1}{B}} (g_{21,2} + g_{21,2} - \underbrace{g_{22,1}}_{2r}) = -\frac{r}{B} ~,
        \end{equation*}

        \begin{equation*}
            \Gamma^1_{33} = \frac{1}{2} g^{1l} (g_{3l,3} + g_{3l,3} - g_{33,l}) =  \frac{1}{2} \underbrace{g^{11}}_{\frac{1}{B}} (g_{31,3} + g_{31,3} - \underbrace{g_{33,1}}_{2 r \sin^2 \theta}) = - \frac{r \sin^2 \theta}{B} ~,
        \end{equation*}

        \begin{equation*}
            \Gamma^1_{01} = \Gamma^1_{10} = \frac{1}{2} g^{1l} (g_{1l,0} + g_{0l,1} - g_{10,l}) =  \frac{1}{2} g^{11} (g_{11,0} + g_{01,1} - g_{10,1}) = 0 ~,
        \end{equation*}

        \begin{equation*}
            \Gamma^1_{02} = \Gamma^1_{20} = \frac{1}{2} g^{1l} (g_{2l,0} + g_{0l,2} - g_{20,l}) =  \frac{1}{2} g^{11} (g_{21,0} + g_{01,2} - g_{20,1}) = 0 ~,
        \end{equation*}

        \begin{equation*}
            \Gamma^1_{03} = \Gamma^1_{30} = \frac{1}{2} g^{1l} (g_{3l,0} + g_{0l,3} - g_{30,l}) =  \frac{1}{2} g^{11} (g_{31,0} + g_{01,3} - g_{30,1}) = 0 ~,
        \end{equation*}

        \begin{equation*}
            \Gamma^1_{12} = \Gamma^1_{21} = \frac{1}{2} g^{1l} (g_{2l,1} + g_{1l,2} - g_{21,l}) =  \frac{1}{2} g^{11} (g_{21,1} + g_{11,2} - g_{21,1}) = 0 ~,
        \end{equation*}
        
        \begin{equation*}
            \Gamma^1_{13} = \Gamma^1_{31} = \frac{1}{2} g^{1l} (g_{3l,1} + g_{1l,3} - g_{31,l}) =  \frac{1}{2} g^{11} (g_{31,1} + g_{11,3} - g_{31,1}) = 0 ~,
        \end{equation*}

        \begin{equation*}
            \Gamma^1_{23} = \Gamma^1_{32} = \frac{1}{2} g^{1l} (g_{3l,2} + g_{2l,3} - g_{32,l}) =  \frac{1}{2} g^{11} (g_{31,2} + g_{21,3} - g_{32,1}) = 0 ~.
        \end{equation*}
        
        The $2$-nd Christoffel symbols are

        \begin{equation*}
            \Gamma^2_{00} = \frac{1}{2} g^{2l} (g_{0l,0} + g_{0l,0} - g_{00,l}) =  \frac{1}{2} g^{22} (g_{02,0} + g_{02,0} - g_{00,2}) = 0 ~,
        \end{equation*}

        \begin{equation*}
            \Gamma^2_{11} = \frac{1}{2} g^{2l} (g_{1l,1} + g_{1l,1} - g_{11,l}) =  \frac{1}{2} g^{22} (g_{12,1} + g_{12,1} - g_{11,2}) = 0 ~, 
        \end{equation*}

        \begin{equation*}
            \Gamma^2_{22} = \frac{1}{2} g^{2l} (g_{2l,2} + g_{2l,2} - g_{22,l}) =  \frac{1}{2} g^{22} (g_{22,2} + g_{22,2} - g_{22,2}) = 0 ~,
        \end{equation*}

        \begin{equation*}
            \Gamma^2_{33} = \frac{1}{2} g^{2l} (g_{3l,3} + g_{3l,3} - g_{33,l}) =  \frac{1}{2} \underbrace{g^{22}}_{\frac{1}{r^2}} (g_{32,3} + g_{32,3} - \underbrace{g_{33,2}}_{2 r^2 \sin \theta \cos \theta}) = - \sin \theta \cos \theta ~, 
        \end{equation*}

        \begin{equation*}
            \Gamma^2_{01} = \Gamma^2_{10} = \frac{1}{2} g^{2l} (g_{1l,0} + g_{0l,1} - g_{10,l}) =  \frac{1}{2} g^{22} (g_{12,0} + g_{02,1} - g_{10,2}) = 0 ~, 
        \end{equation*}

        \begin{equation*}
            \Gamma^2_{02} = \Gamma^2_{20} = \frac{1}{2} g^{2l} (g_{2l,0} + g_{0l,2} - g_{20,l}) =  \frac{1}{2} g^{22} (g_{22,0} + g_{02,2} - g_{20,2}) = 0 ~,
        \end{equation*}

        \begin{equation*}
            \Gamma^2_{03} = \Gamma^2_{30} = \frac{1}{2} g^{2l} (g_{3l,0} + g_{0l,3} - g_{30,l}) =  \frac{1}{2} g^{22} (g_{32,0} + g_{02,3} - g_{30,2}) = 0 ~,
        \end{equation*}

        \begin{equation*}
            \Gamma^2_{12} = \Gamma^2_{21} = \frac{1}{2} g^{2l} (g_{2l,1} + g_{1l,2} - g_{21,l}) =  \frac{1}{2} \underbrace{g^{22}}_{\frac{1}{r^2}} (\underbrace{g_{22,1}}_{2r} + g_{12,2} - g_{21,2}) = \frac{1}{r} ~,
        \end{equation*}

        \begin{equation*}
            \Gamma^2_{13} = \Gamma^2_{31} = \frac{1}{2} g^{2l} (g_{3l,1} + g_{1l,3} - g_{31,l}) =  \frac{1}{2} g^{22} (g_{32,1} + g_{12,3} - g_{31,2}) = 0 ~, 
        \end{equation*}

        \begin{equation*}
            \Gamma^2_{23} = \Gamma^2_{32} = \frac{1}{2} g^{2l} (g_{3l,2} + g_{2l,3} - g_{32,l}) =  \frac{1}{2} g^{22} (g_{32,2} + g_{22,3} - g_{32,2}) = 0 ~. 
        \end{equation*}

        The $3$-rd Christoffel symbols are

        \begin{equation*}
            \Gamma^3_{00} = \frac{1}{2} g^{3l} (g_{0l,0} + g_{0l,0} - g_{00,l}) = \frac{1}{2} g^{33} (g_{03,0} + g_{03,0} - g_{00,3}) = 0 ~,
        \end{equation*}

        \begin{equation*}
            \Gamma^3_{11} = \frac{1}{2} g^{3l} (g_{1l,1} + g_{1l,1} - g_{11,l}) = \frac{1}{2} g^{33} (g_{13,1} + g_{13,1} - g_{11,3}) = 0 ~,
        \end{equation*}

        \begin{equation*}
            \Gamma^3_{22} = \frac{1}{2} g^{3l} (g_{2l,2} + g_{2l,2} - g_{22,l}) = \frac{1}{2} g^{33} (g_{23,2} + g_{23,2} - g_{22,3}) = 0 ~,
        \end{equation*}

        \begin{equation*}
            \Gamma^3_{33} = \frac{1}{2} g^{3l} (g_{3l,3} + g_{3l,3} - g_{33,l}) = \frac{1}{2} g^{33} (g_{33,3} + g_{33,3} - g_{33,3}) = 0 ~,
        \end{equation*}

        \begin{equation*}
            \Gamma^3_{01} = \Gamma^3_{10} = \frac{1}{2} g^{3l} (g_{1l,0} + g_{0l,1} - g_{10,l}) = \frac{1}{2} g^{33} (g_{13,0} + g_{03,1} - g_{10,3}) = 0 ~,
        \end{equation*}

        \begin{equation*}
            \Gamma^3_{02} = \Gamma^3_{20} = \frac{1}{2} g^{3l} (g_{2l,0} + g_{0l,2} - g_{20,l}) = \frac{1}{2} g^{33} (g_{23,0} + g_{03,2} - g_{20,3}) = 0 ~, 
        \end{equation*}

        \begin{equation*}
            \Gamma^3_{03} = \Gamma^3_{30} = \frac{1}{2} g^{3l} (g_{3l,0} + g_{0l,3} - g_{30,l}) = \frac{1}{2} g^{33} (g_{33,0} + g_{03,3} - g_{30,3}) = 0 ~,
        \end{equation*}

        \begin{equation*}
            \Gamma^3_{12} = \Gamma^3_{21} = \frac{1}{2} g^{3l} (g_{2l,1} + g_{1l,2} - g_{21,l}) = \frac{1}{2} g^{33} (g_{23,1} + g_{13,2} - g_{21,3}) = 0 ~,
        \end{equation*}

        \begin{equation*}
            \Gamma^3_{13} = \Gamma^3_{31} = \frac{1}{2} g^{3l} (g_{3l,1} + g_{1l,3} - g_{31,l}) = \frac{1}{2} \underbrace{g^{33}}_{\frac{1}{r^2 \sin^2 \theta}} (\underbrace{g_{33,1}}_{2 r \sin^2 \theta} + g_{13,3} - g_{31,3}) = \frac{1}{r} ~,
        \end{equation*}

        \begin{equation*}
            \Gamma^3_{23} = \Gamma^3_{32} = \frac{1}{2} g^{3l} (g_{3l,2} + g_{2l,3} - g_{32,l}) = \frac{1}{2} \underbrace{g^{33}}_{\frac{1}{r^2 \sin^2 \theta}} (\underbrace{g_{33,2}}_{2 r^2 \sin \theta \cos \theta} + g_{23,3} - g_{32,3}) = \frac{\cos \theta}{\sin \theta} ~.
        \end{equation*}

        Hence, the non-zero Christoffel symbols are 
        \begin{equation*}
            \Gamma^0_{01} = \Gamma^0_{10} = \frac{A'}{2A} ~, \quad \Gamma^1_{00} = - \frac{A'}{2B} ~, \quad \Gamma^1_{11} = \frac{B'}{2B} ~, \quad \Gamma^1_{22} = - \frac{r}{B} ~, \quad \Gamma^1_{33} = - \frac{r \sin^2 \theta}{B} ~,
        \end{equation*}
        \begin{equation*}
            \Gamma^2_{33} = - \sin\theta \cos\theta ~, \quad \Gamma^2_{12} =  \Gamma^2_{21} = \frac{1}{r} ~, \quad \Gamma^3_{13} = \Gamma^3_{31} = \frac{1}{r} ~, \quad \Gamma^3_{23} = -\frac{\cos \theta}{\sin \theta} ~. 
        \end{equation*}

        The derivatives are 

        \begin{equation*}
            \Gamma^0_{01,1} = \Gamma^0_{10,1} = \pdv{}{r} \Big (\frac{A'}{2A} \Big) = \frac{A''A - (A')^2}{2A^2} ~,
        \end{equation*}

        \begin{equation*}
            \Gamma^1_{00,1} = \pdv{}{r} \Big ( - \frac{A'}{2B} \Big) = - \frac{A'' B - A' B'}{2B^2} ~,
        \end{equation*}

        \begin{equation*}
            \Gamma^1_{11,1} = \pdv{}{r} \Big (\frac{B'}{2B} \Big) = \frac{B''B - (B')^2}{2B^2} ~,
        \end{equation*}

        \begin{equation*}
            \Gamma^1_{22,1} = \pdv{}{r} \Big (- \frac{r}{B} \Big) = -\frac{B - r B'}{B^2} ~,
        \end{equation*}

        \begin{equation*}
            \Gamma^1_{33,1} = \pdv{}{r} \Big ( - \frac{r \sin^2 \theta}{B} \Big) = - \sin^2 \theta \frac{B - rB'}{B^2} ~,
        \end{equation*}

        \begin{equation*}
            \Gamma^1_{33,2} = \pdv{}{\theta} \Big ( - \frac{r \sin^2 \theta}{B} \Big) = - \frac{2 r \sin \theta \cos \theta}{B^2} ~,
        \end{equation*}

        \begin{equation*}
            \Gamma^2_{33,2} = \pdv{}{\theta} ( \sin \theta \cos \theta ) = \cos^2 \theta - \sin^2 \theta ~,
        \end{equation*}

        \begin{equation*}
            \Gamma^2_{12,1} = \Gamma^2_{21,1} = \pdv{}{r} \Big ( \frac{1}{r}\Big)  = - \frac{1}{r^2} ~,
        \end{equation*}

        \begin{equation*}
            \Gamma^3_{13,1} = \Gamma^3_{31,1} = \pdv{}{r} \Big ( \frac{1}{r} \Big) = - \frac{1}{r^2} ~,
        \end{equation*}

        \begin{equation*}
            \Gamma^3_{23,2} = \pdv{}{\theta} \cot \theta = - \frac{1}{\sin^2 \theta} ~.
        \end{equation*}

        The Ricci tensor is 
        \begin{equation*}
            R_{ij} = \Gamma^k_{ij,k} - \Gamma^k_{ik,j} + \Gamma^a_{ij} \Gamma^k_{ak} - \Gamma^a_{ik} \Gamma^k_{aj} ~.
        \end{equation*}

        Its components are

        \begin{equation*}
        \begin{aligned}
            R_{00} & = \Gamma^k_{00,k} - \Gamma^k_{0k,0} + \Gamma^a_{00} \Gamma^k_{ak} - \Gamma^a_{0k} \Gamma^k_{a0} \\ & =  \Gamma^1_{00,1} + \Gamma^1_{00} \Gamma^0_{10} + \Gamma^1_{00} \Gamma^1_{11} + \Gamma^1_{00} \Gamma^2_{12} + \Gamma^1_{00} \Gamma^3_{13} - \Gamma^0_{01} \Gamma^1_{00} - \Gamma^1_{00} \Gamma^0_{10} \\ & = - \frac{A''B - A' B'}{2B^2} - \cancel{\frac{A'}{2B} \frac{A'}{2A}} - \frac{A'}{2B} \frac{B'}{2B} - \frac{A'}{2rB} - \frac{A'}{2rB} + \frac{A'}{2A} \frac{A'}{2B} + \cancel{\frac{A'}{2B} \frac{A'}{2A}} \\ & = - \frac{A''}{2B} + \frac{A'B'}{4B^2} - \frac{A'}{rB} + \frac{(A')^2}{4 AB} ~,
        \end{aligned}
        \end{equation*}

        \begin{equation*}
        \begin{aligned}
            R_{11} & = \Gamma^k_{11,k} - \Gamma^k_{1k,1} + \Gamma^a_{11} \Gamma^k_{ak} - \Gamma^a_{1k} \Gamma^k_{a1} \\ & = \cancel{\Gamma^1_{11,1}} - \Gamma^0_{10,1} - \cancel{\Gamma^1_{11,1} } - \Gamma^2_{12,1} - \Gamma^3_{13,1} + \Gamma^1_{11} \Gamma^0_{10} + \cancel{\Gamma^1_{11} \Gamma^1_{11}} \\ & \quad  + \Gamma^1_{11} \Gamma^2_{12}  + \Gamma^1_{11} \Gamma^3_{13} - \Gamma^0_{10} \Gamma^0_{01}  - \cancel{\Gamma^1_{11} \Gamma^1_{11}}  - \Gamma^2_{12} \Gamma^2_{21} - \Gamma^3_{13} \Gamma^3_{31}  \\ & = - \frac{A''A - (A'^2)}{2A^2} + \cancel{\frac{1}{r^2}} + \cancel{\frac{1}{r^2}} + \frac{B'}{2B} \frac{A'}{2A} + \frac{B'}{2rB} + \frac{B'}{2rB} - \frac{(A')^2}{4A^2} - \cancel{\frac{1}{r^2}} - \cancel{\frac{1}{r^2}} \\ & = - \frac{A''}{2A} + \frac{(A')^2}{4A^2} + \frac{B'A'}{4AB} + \frac{B'}{rB} ~, 
        \end{aligned}
        \end{equation*}

        \begin{equation*}
        \begin{aligned}
            R_{22} & = \Gamma^k_{22,k} - \Gamma^k_{2k,2} + \Gamma^a_{22} \Gamma^k_{ak} - \Gamma^a_{2k} \Gamma^k_{a2} \\ & = \Gamma^1_{22,1} - \Gamma^3_{23,2} + \Gamma^1_{22} \Gamma^0_{10} + \Gamma^1_{22} \Gamma^1_{11} + \cancel{\Gamma^1_{22} \Gamma^2_{12}} \\ & \quad + \Gamma^1_{22} \Gamma^3_{13} - \cancel{\Gamma^1_{22} \Gamma^2_{12}} - \Gamma^2_{21} \Gamma^1_{22} - \Gamma^3_{23} \Gamma^3_{32} \\ & = - \frac{B-rB'}{B^2} + \frac{1}{\sin^2 \theta}  - \frac{r}{B} \frac{A'}{2A} - \frac{r}{B} \frac{B'}{2B} - \cancel{\frac{r}{B} \frac{1}{r}} + \cancel{\frac{1}{r} \frac{r}{B}} - \cot^2 \theta \\ & = 1 - \frac{1}{B} + \frac{rB'}{2B^2} - \frac{rA'}{2AB} ~, 
        \end{aligned}
        \end{equation*}

        \begin{equation*}
        \begin{aligned}
            R_{33} & = \Gamma^k_{33,k} - \Gamma^k_{3k,3} + \Gamma^a_{33} \Gamma^k_{ak} - \Gamma^a_{3k} \Gamma^k_{a3} \\ & =\Gamma^1_{33,1} + \Gamma^2_{33,2} + \Gamma^1_{33} \Gamma^0_{10} + \Gamma^1_{33} \Gamma^1_{11} + \Gamma^1_{33} \Gamma^2_{12} + \cancel{\Gamma^2_{33} \Gamma^3_{23}} + \cancel{\Gamma^1_{33} \Gamma^3_{13}} - \cancel{\Gamma^1_{33} \Gamma^3_{13} } - \cancel{\Gamma^2_{33} \Gamma^3_{23}} - \Gamma^3_{31} \Gamma^1_{33} - \Gamma^3_{32} \Gamma^2_{33} \\ & = - \sin^2 \theta \frac{B-rB'}{B^2} + \cancel{\cos^2 \theta} - \sin^2 \theta - \frac{r \sin^2 \theta}{B} \frac{A'}{2A} - \frac{r \sin^2 \theta}{B} \frac{B'}{2B} - \cancel{\frac{r \sin^2 \theta}{B} \frac{1}{r}} \\ & \quad - \cancel{\frac{1}{r} \frac{r \sin^2 \theta}{B}} - \cancel{\frac{\cos \theta}{\sin \theta} \sin \theta \cos \theta} \\ & = \sin^2 \theta - \sin^2 \theta \frac{1}{B} + \sin^2 \theta \frac{rB'}{2B^2} - \sin^2 \theta \frac{rA'}{2AB} \\ & = \sin^2 \theta R_{22} ~.
        \end{aligned}
        \end{equation*}

        Finally, we find a system of differential equations 
        \begin{equation*}
        \begin{aligned}
            & R_{00} = - \frac{A''}{2B} + \frac{(A')^2}{4 AB} + \frac{A'B'}{4B^2} - \frac{A'}{rB}  = 0 ~,
            \\ & R_{11} = - \frac{A''}{2A} + \frac{(A')^2}{4A^2} + \frac{B'A'}{4AB} + \frac{B'}{rB} = 0 ~,
            \\ & R_{22} = 1 - \frac{1}{B} + \frac{rB'}{2B^2} - \frac{rA'}{2AB} = 0 ~,
            \\ & R_{33} = \sin^2 \theta R_{22} = 0 ~.
        \end{aligned}
        \end{equation*}

        We notice that
        \begin{equation*}
        \begin{aligned}
            0 & = \frac{B}{A} R_{00} - R_{11} \\ & = - \cancel{\frac{B}{A} \frac{A''}{2B}} + \cancel{\frac{B}{A} \frac{(A')^2}{4 AB}} + \cancel{ \frac{B}{A} \frac{A'B'}{4B^2}} - \frac{B}{A} \frac{A'}{rB} + \cancel{\frac{A''}{2A}} - \cancel{\frac{(A')^2}{4A^2}} - \cancel{\frac{B'A'}{4AB}} - \frac{B'}{rB} \\ & = - \frac{A'}{rA} - \frac{B'}{rB} ~.
        \end{aligned}
        \end{equation*}
        Hence 
        \begin{equation*}
            0 = A' B + B' A = (AB)' ~,
        \end{equation*}
        which implies, after a time rescaling, that 
        \begin{equation*}
            A = - B^{-1} ~.
        \end{equation*}

        Therefore, the third equation becomes 
        \begin{equation*}
            0 = 1 - \frac{1}{B} + \frac{rB'}{2B^2} - \frac{rA'}{2AB} = 1 + A - rA, ~,
        \end{equation*}
        or, equivalently, 
        \begin{equation*}
            (rA)' = 1 ~. 
        \end{equation*}

        Its solution is 
        \begin{equation*}
            A = 1 - \frac{2}{}
        \end{equation*}
    \end{proof}